fsafas

meta_subst_type_assign.v
@@ -4,15 +4,15 @@ Require Import type_assign.
 Require Import meta_subst.
 Require Import comp_expr.
 Require Import meta_subst_type.
- Fixpoint app_msubst_tp_assign' {W G'} (G:tp_assign W G') : forall {W'} (theta:msubst W W'), tp_assign W' G' :=
+ Fixpoint app_msubst_tp_assign' {W G'} (G:tp_assign G' W) : forall {W'} (theta:msubst W W'), tp_assign G' W' :=
   match G in star _ _ G' return forall {W'} (theta:msubst W W'), star (var_tp W') empty G' with
    | s_nil => fun W' theta => s_nil
    | s_cons _ _ a (b,c) => fun W' theta => s_cons _ (app_msubst_tp_assign' a _ theta) (b,app_msubst_t2 theta c)
   end.
  
- Definition app_msubst_tp_assign {G' W W'} (theta:msubst W W') (G:tp_assign W G') : tp_assign W' G' := app_msubst_tp_assign' G _ theta.
+ Definition app_msubst_tp_assign {G' W W'} (theta:msubst W W') (G:tp_assign G' W) : tp_assign G' W' := app_msubst_tp_assign' G _ theta.
  Definition tp_assign' δ γ := tp_assign γ δ.
- Instance tp_assign_substitutable γ : substitutable (tp_assign' γ) := (@app_msubst_tp_assign γ).
+ Instance tp_assign_substitutable γ : substitutable (tp_assign γ) := (@app_msubst_tp_assign γ).
 
  Instance tp_substitutable : substitutable tp := @app_msubst_t2.
 
