type_assign.v
@@ -4,15 +4,15 @@ Require Import comp_expr.
 
 Open Scope type_scope. 
 Definition var_tp D G1 G2 := (slink G1 G2)*(tp D).
- Definition tp_assign D := star (var_tp D) empty.
+ Definition tp_assign G D := star (var_tp D) empty G.
  Definition tp_assign_nil D := @s_nil _ (var_tp D).
  Definition v_cons D := @s_cons _ (var_tp D) empty.
  Implicit Arguments v_cons.
  Print Implicit v_cons.
 
  (* TODO: We could eliminate the duplication between this and the other one *)
- Inductive var_assigned D G : tp_assign D G -> name G -> tp D -> Prop :=
-  | v_asn_top : forall G' (A:tp_assign D G') T x,
+ Inductive var_assigned D G : tp_assign G D -> name G -> tp D -> Prop :=
+  | v_asn_top : forall G' (A:tp_assign G' D) T x,
                     var_assigned D G (v_cons A (x,T)) x T
   | v_asn_else : forall G' T A x (y:slink G' G) U,
                  var_assigned D G' A x T
